updating Surface.Term

Surface/Term/Definition.lean
@@ -3,6 +3,7 @@ import Surface.Ty
 import Core.Vec
 
 open LeanSubst
+open Lilac
 
 namespace Surface
 
@@ -13,7 +14,7 @@ inductive Term : Type where
 | app : Term -> Term -> Term
 | lamt :  Kind -> Term -> Term
 | lam : Ty -> Term -> Term
-| «match» : (n : Nat) -> Ty -> Term -> Vect n Term -> Vect n Term -> Term -> Term
+-- | «match» : (n : Nat) -> Ty -> Term -> Fun.Vec Term n -> Fun.Vec Term n -> Term -> Term
 | annot : Term -> Ty -> Term
 
 
@@ -29,7 +30,7 @@ notation:70 f " `• " a:70 => Term.app f a
 notation "Λˢ[" K "]" t => Term.lamt K t
 notation "λˢ[" A "]" t => Term.lam A t
 
-notation "matchˢ!" => Term.match
+-- notation "matchˢ!" => Term.match
 
 
 protected def Term.repr (p : Nat) : (a : Term) -> Std.Format
@@ -42,16 +43,16 @@ protected def Term.repr (p : Nat) : (a : Term) -> Std.Format
 | .lamt K t =>
   Repr.addAppParen ("Λˢ" ++ Std.Format.sbracket (repr K) ++ " " ++ Term.repr max_prec t) p
 | .lam τ t => Repr.addAppParen ("λˢ" ++ Std.Format.sbracket (repr τ) ++ " " ++ Term.repr max_prec t) p
-| .match n _ s pats ts d =>
-  let ts : Vect n Std.Format := λ i =>
-    let t := ts i
-    let pat := pats i
-    Std.Format.nest 4 <| Std.Format.line ++ Term.repr p pat ++ " -> " ++ Term.repr p t
-  let css := Vect.fold Std.Format.nil (·++·) ts
-  Std.Format.nest 4 <| (("match " ++ Term.repr max_prec s ++ " with")
-    ++ css
-    ++ (Std.Format.nest 4 <| Std.Format.line ++ " _ ->> " ++ Term.repr p d)
-    )
+-- | .match n _ s pats ts d =>
+--   let ts : Fun.Vec Std.Format n := λ i =>
+--     let t := ts i
+--     let pat := pats i
+--     Std.Format.nest 4 <| Std.Format.line ++ Term.repr p pat ++ " -> " ++ Term.repr p t
+--   let css := ts.to.foldl (·++·) Std.Format.nil
+--   Std.Format.nest 4 <| (("match " ++ Term.repr max_prec s ++ " with")
+--     ++ css
+--     ++ (Std.Format.nest 4 <| Std.Format.line ++ " _ -> " ++ Term.repr p d)
+--     )
 | annot t ty =>
   Std.Format.paren (Term.repr p t ++ " : " ++ repr ty)
 
@@ -67,10 +68,8 @@ def Term.size : Term -> Nat
 | appt t1 _ => size t1 + 1
 | lamt _ t => size t + 1
 | lam _ t => size t + 1
-| «match» _ _ t1 t2 t3 t4 =>
-  let t2' : Vect _ _ := size <$> t2
-  let t3' : Vect _ _ := size <$> t3
-  size t1 + List.sum t2' + List.sum t3' + size t4 + 1
+-- | «match» _ _ t1 t2 t3 t4 =>
+--  size t1 + t2.to.length + t3.to.length + size t4 + 1
 | annot t _ => size t + 1
 
 end Surface
