Surface/Term/Substitution.lean
@@ -7,16 +7,16 @@ open LeanSubst
 namespace Surface
 
 @[coe]
-def Term.from_action : Subst.Action Term -> Term
+def Term.from_action : Action Term -> Term
 | .re y => `#y
 | .su t => t
 
 @[simp]
-theorem Term.from_action_id {n} : from_action (+0 n) = `#n := by
+theorem Term.from_action_id {n} : from_action (+0σ.act n) = `#n := by
   simp [from_action, Subst.id]
 
 @[simp]
-theorem Term.from_action_succ {n} : from_action (+1 n) = `#(n + 1) := by
+theorem Term.from_action_succ {n} : from_action (+1σ.act n) = `#(n + 1) := by
   simp [from_action, Subst.succ]
 
 @[simp]
@@ -25,46 +25,84 @@ theorem Term.from_acton_re {n} : from_action (re n) = `#n := by simp [from_actio
 @[simp]
 theorem Term.from_action_su {t} : from_action (su t) = t := by simp [from_action]
 
-instance instCoe_ActionTermTerm : Coe (Subst.Action Term) Term where
+instance instCoe_ActionTermTerm : Coe (Action Term) Term where
   coe := Term.from_action
 
 @[simp]
-def Term.rmap (r : Ren) : Term -> Term
-| `#x => `#(r x)
+def Term.rmap (r : Ren Term) : Term -> Term
+| `#x => `#(r.act x)
 | g`#x => g`#x
 | lamt A t => lamt A (rmap r t)
 | lam A t => lam A (rmap r.lift t)
 | app t1 t2 => app (rmap r t1) (rmap r t2)
 | appt t1 t2 => appt (rmap r t1) t2
-| .match n t0 t1 t2 t3 t4 => .match n t0 (rmap r t1) (rmap r <$> t2) (rmap r <$> t3) (rmap r t4)
+-- | .match n t0 t1 t2 t3 t4 => .match n t0 (rmap r t1) (rmap r <$> t2) (rmap r <$> t3) (rmap r t4)
 | annot t1 A => annot (rmap r t1) A
 
-instance instRenMap_Term : RenMap Term where
+instance instRenMap_Term : RenMap Term Term where
   rmap := Term.rmap
+
+@[simp]
+def Term.Ty.rmap (r : Ren Ty) : Term -> Term
+| `#x => `#x
+| g`#x => g`#x
+| lamt A t => lamt A (rmap r.lift t)
+| lam A t => lam A⟨r⟩ (rmap r t)
+| app t1 t2 => app (rmap r t1) (rmap r t2)
+| appt t1 t2 => appt (rmap r t1) t2⟨r⟩
+-- | .match m t0 t1 t2 t3 t4 =>  .match m t0⟨r⟩ (rmap r t1) (rmap r <$> t2) (rmap r <$> t3) (rmap r t4)
+| annot t1 A => annot (rmap r t1) A⟨r⟩
+
+instance : RenMap Term Ty where
+  rmap := Term.Ty.rmap
 
 @[simp]
 def Term.Ty.smap (σ : Subst Ty) : Term -> Term
 | `#x => `#x
 | g`#x => g`#x
 | app t1 t2 => app (smap σ t1) (smap σ t2)
-| appt t1 t2 => appt (smap σ t1) t2[σ:_]
+| appt t1 t2 => appt (smap σ t1) t2[σ]
 | lamt A t => lamt A (smap σ.lift t)
-| lam A t => lam A[σ:_] (smap σ t)
-| .match n t0 t1 t2 t3 t4  => .match n t0 (smap σ t1) (λ i => smap σ (t2 i)) (λ i => smap σ (t3 i)) (smap σ t4)
-| annot t1 A => annot (smap σ t1) A[σ:_]
+| lam A t => lam A[σ] (smap σ t)
+-- | .match n t0 t1 t2 t3 t4  => .match n t0 (smap σ t1) (λ i => smap σ (t2 i)) (λ i => smap σ (t3 i)) (smap σ t4)
+| annot t1 A => annot (smap σ t1) A[σ]
 
 instance instSubstMap_TermTy : SubstMap Term Ty where
   smap := Term.Ty.smap
 
 @[simp]
+theorem Term.ren_var {r : Ren Term} : (`#x)⟨r⟩ = `#(r.act x) := by
+  simp [RenMap.rmap]
+
+@[simp]
+theorem Term.ren_global {r : Ren Term} : (g`#x)⟨r⟩ = g`#x := by
+  simp [RenMap.rmap]
+
+@[simp]
+theorem Term.ren_lam {r : Ren Term} : (lam A t)⟨r⟩ = lam A t⟨r.lift⟩ := by
+  simp [RenMap.rmap]
+
+@[simp]
+theorem Term.ren_lamt {r : Ren Term} : (lamt A t)⟨r⟩ = lamt A t⟨r⟩ := by
+  simp [RenMap.rmap]
+
+-- @[simp]
+-- theorem Term.ren_match {r : Ren Term}
+--   : (.match n t0 t1 t2 t3 t4)⟨r⟩
+--     = .match n (λ i => (t1 i)⟨r⟩) t2 (λ i => (t3 i)⟨r.lift (t2 i).bind⟩)
+-- := by
+--   simp [RenMap.rmap]
+
+
+@[simp]
 def Term.smap (σ : Subst Term) : Term -> Term
-| `#x => σ x
+| `#x => σ.act x
 | g`#x => g`#x
 | app t1 t2 => app (smap σ t1) (smap σ t2)
 | appt t1 t2 => appt (smap σ t1) t2
-| lamt A t => lamt A (smap (σ ◾ +1@Ty) t)
+| lamt A t => lamt A (smap (σ ◾ Ren.succ Ty) t)
 | lam A t => lam A (smap σ.lift t)
-| .match n t0 t1 t2 t3 t4 => .match n t0 (smap σ t1) (λ i => smap σ (t2 i)) (λ i => smap σ (t3 i)) (smap σ t4)
+-- | .match n t0 t1 t2 t3 t4 => .match n t0 (smap σ t1) (λ i => smap σ (t2 i)) (λ i => smap σ (t3 i)) (smap σ t4)
 | annot t1 A => annot (smap σ t1) A
 
 
@@ -73,150 +111,141 @@ instance instSubstMap_TermTerm : SubstMap Term Term where
   smap := Term.smap
 
 @[simp]
-theorem Term.subst_var : (`#x)[σ:Term] = σ x := by
+theorem Term.subst_var {σ : Subst Term} : (`#x)[σ] = σ.act x := by
   simp [SubstMap.smap]
 
 @[simp]
-theorem Term.subst_global : (g`#x)[σ:Term] = g`#x := by
+theorem Term.subst_global {σ : Subst Term} : (g`#x)[σ] = g`#x := by
   simp [SubstMap.smap]
 
 @[simp]
-theorem Term.subst_app : (app t1 t2)[σ:Term] = app t1[σ:_] t2[σ:_] := by
+theorem Term.subst_app {σ : Subst Term} : (app t1 t2)[σ] = app t1[σ] t2[σ] := by
   simp [SubstMap.smap]
 
 @[simp]
-theorem Term.subst_appt : (appt t1 t2)[σ:Term] = appt t1[σ:_] t2 := by
+theorem Term.subst_appt {σ : Subst Term} : (appt t1 t2)[σ] = appt t1[σ] t2 := by
   simp [SubstMap.smap]
 
 @[simp]
-theorem Term.subst_annoτ : (annot t1 t2)[σ:Term] = annot t1[σ:_] t2 := by
+theorem Term.subst_annoτ {σ : Subst Term} : (annot t1 t2)[σ] = annot t1[σ] t2 := by
   simp [SubstMap.smap]
 
 
 @[simp]
-theorem Term.subst_lamt : (lamt A t)[σ:Term] = lamt A t[σ ◾ +1@Ty:_] := by
+theorem Term.subst_lamt {σ : Subst Term} : (lamt A t)[σ] = lamt A t[σ ◾ Ren.succ Ty] := by
   simp [SubstMap.smap]
 
 @[simp]
-theorem Term.subst_lam : (lam A t)[σ:Term] = lam A t[σ.lift:_] := by
+theorem Term.subst_lam {σ : Subst Term} : (lam A t)[σ] = lam A t[σ.lift] := by
   simp [SubstMap.smap]
 
-@[simp]
-theorem Term.subst_match
-  : (matchˢ! n t0 t1 t2 t3 t4)[σ:Term] = matchˢ! n t0 t1[σ:_] (λ i => (t2 i)[σ:_]) (λ i => (t3 i)[σ:_]) (t4[σ:_])
-:= by
-  simp [SubstMap.smap]
+-- @[simp]
+-- theorem Term.subst_match {σ : Subst Term}
+--   : (matchˢ! n t0 t1 t2 t3 t4)[σ] = matchˢ! n t0 t1[σ] (λ i => (t2 i)[σ]) (λ i => (t3 i)[σ]) (t4[σ])
+-- := by
+--   simp [SubstMap.smap]
 
 @[simp]
-theorem Term.from_action_compose {x} {σ τ : Subst Term}
-  : (from_action (σ x))[τ] = from_action ((σ ∘ τ) x)
+theorem Term.from_action_compose {x : Nat} {σ τ : Subst Term}
+  : (from_action (σ.act x))[τ] = from_action ((σ ∘ τ).act x)
 := by
   simp [Term.from_action, Subst.compose]
-  generalize zdef : σ x = z
+  generalize zdef : σ.act x = z
   cases z <;> simp [Term.from_action]
 
 @[simp]
-theorem Term.Ty.subst_var : (`#x)[σ:Ty] = `#x := by
-  simp [SubstMap.smap]
-
-@[simp]
-theorem Term.Ty.subst_global : (g`#x)[σ:Ty] = g`#x := by
-  simp [SubstMap.smap]
-
-@[simp]
-theorem Term.Ty.subst_app : (app t1 t2)[σ:Ty] = app t1[σ:_] t2[σ:_] := by
-  simp [SubstMap.smap]
-@[simp]
-theorem Term.Ty.subst_appt : (appt t1 t2)[σ:Ty] = appt t1[σ:_] t2[σ:_] := by
-  simp [SubstMap.smap]
-
-@[simp]
-theorem Term.Ty.subst_lamt : (lamt A t)[σ:Ty] = lamt A t[σ.lift:_] := by
-  simp [SubstMap.smap]
-
-@[simp]
-theorem Term.Ty.subst_lam : (lam A t)[σ:Ty] = lam A[σ:_] t[σ:_] := by
-  simp [SubstMap.smap]
-
-@[simp]
-theorem Term.Ty.subst_annoτ : (annot t A)[σ:Ty] = annot t[σ:_] A[σ:_] := by
-  simp [SubstMap.smap]
+theorem Term.Ty.ren_var {r : Ren Ty} : (`#x)⟨r⟩ = `#x := by simp [RenMap.rmap]
 
 
 @[simp]
-theorem Term.Ty.subst_match
-  : (matchˢ! n t0 t1 ps t2 t3)[σ:Ty] = matchˢ! n t0 t1[σ:_] (λ i => (ps i)[σ:_]) (λ i => (t2 i)[σ:_]) t3[σ:_]
-:= by
+theorem Term.Ty.subst_var {σ : Subst Ty} : (`#x)[σ] = `#x := by
   simp [SubstMap.smap]
 
-theorem Term.Ty.apply_id {t : Term} : t[+0:Ty] = t := by
-  induction t
-  all_goals (simp at * <;> try simp [*])
+@[simp]
+theorem Term.Ty.subst_global {σ : Subst Ty} : (g`#x)[σ] = g`#x := by
+  simp [SubstMap.smap]
+
+@[simp]
+theorem Term.Ty.subst_app {σ : Subst Ty} : (app t1 t2)[σ] = app t1[σ] t2[σ] := by
+  simp [SubstMap.smap]
+@[simp]
+theorem Term.Ty.subst_appt {σ : Subst Ty} : (appt t1 t2)[σ] = appt t1[σ] t2[σ] := by
+  simp [SubstMap.smap]
+
+@[simp]
+theorem Term.Ty.subst_lamt {σ : Subst Ty} : (lamt A t)[σ] = lamt A t[σ.lift] := by
+  simp [SubstMap.smap]
+
+@[simp]
+theorem Term.Ty.subst_lam {σ : Subst Ty} : (lam A t)[σ] = lam A[σ] t[σ] := by
+  simp [SubstMap.smap]
+
+@[simp]
+theorem Term.Ty.subst_annoτ {σ : Subst Ty} : (annot t A)[σ] = annot t[σ] A[σ] := by
+  simp [SubstMap.smap]
+
+
+-- @[simp]
+-- theorem Term.Ty.subst_match
+--   : (matchˢ! n t0 t1 ps t2 t3)[σ:Ty] = matchˢ! n t0 t1[σ:_] (λ i => (ps i)[σ:_]) (λ i => (t2 i)[σ:_]) t3[σ:_]
+-- := by
+--   simp [SubstMap.smap]
+
 
 instance instSubstMapId_Ty_TermTy : SubstMapId Term Ty where
-  apply_id := Term.Ty.apply_id
+  apply_id := by subst_solve_id
 
 @[simp]
-theorem Term.hcompose_var {σ : Subst Term} {τ : Subst Ty}
-  : (σ ◾ τ) x = (Term.from_action (σ x))[τ:Ty]
+theorem Term.hcompose_var {x : Nat}{σ : Subst Term} {τ : Subst Ty}
+  : (σ ◾ τ).act x = (Term.from_action (σ.act x))[τ]
 := by
   simp [Subst.hcompose, Term.from_action]
-  generalize zdef : σ x = z
+  generalize zdef : σ.act x = z
   cases z <;> simp
 
-theorem Term.apply_stable (r : Ren) (σ : Subst Term)
-  : r = σ -> rmap r =  smap σ
-:= by subst_solve_stable r, σ
+theorem Term.apply_stable (r : Ren Term) (σ : Subst Term)
+  : r.to = σ -> rmap r =  smap σ
+:= by sorry
 
 
-instance instSubstMapStable_Term : SubstMapStable Term where
+instance instSubstMapStable_Term : SubstMapStable Term Term where
   apply_stable := Term.apply_stable
 
-theorem Term.apply_ren_commute {s : Term} (r : Ren) (τ : Subst Ty)
-  : s[r.to][τ:Ty] = s[τ:Ty][r.to]
-:= by
-  induction s generalizing r τ <;> simp [Ren.to] at *
-  all_goals try simp [*]
-  case lam A t ih =>
-    replace ih := ih r.lift
-    rw [Ren.to_lift] at ih; simp at ih
-    apply ih
+-- theorem Term.apply_ren_commute {s : Term} (r : Ren Ty) (τ : Subst Ty)
+--   : s[r.to][τ] = s[τ][r.to]
+-- := by
+--   induction s generalizing r τ <;> simp [Ren.to] at *
+--   all_goals try simp [*]
+--   case lam A t ih =>
+--     replace ih := ih r.lift
+--     rw [Ren.to_lift] at ih; simp at ih
+--     apply ih
 
-instance instSubstMapRenCommute_Term : SubstMapRenCommute Term Ty where
-  apply_ren_commute := Term.apply_ren_commute
+-- instance instSubstMapRenCommute_Term : SubstMapRenCommute Term Ty where
+--   apply_ren_commute := Term.apply_ren_commute
 
-theorem Term.Ty.apply_compose {s : Term} {σ τ : Subst Ty} : s[σ:Ty][τ:_] = s[σ ∘ τ:_] := by
-  subst_solve_compose Ty, s, σ, τ
+-- theorem Term.Ty.apply_compose {s : Term} {σ τ : Subst Ty} : s[σ:Ty][τ:_] = s[σ ∘ τ:_] := by
+--   subst_solve_compose Ty, s, σ, τ
 
-instance instSubstMapCompose_TermTy : SubstMapCompose Term Ty where
-  apply_compose := Term.Ty.apply_compose
+-- instance instSubstMapCompose_TermTy : SubstMapCompose Term Ty where
+--   apply_compose := Term.Ty.apply_compose
 
-theorem Term.apply_hcompose {s : Term} {σ : Subst Term} {τ : Subst Ty}
-  : s[σ][τ:_] = s[τ:_][σ ◾ τ]
-:= by subst_solve_hcompose Term, Ty, s, σ, τ
+-- theorem Term.apply_hcompose {s : Term} {σ : Subst Term} {τ : Subst Ty}
+--   : s[σ][τ:_] = s[τ:_][σ ◾ τ]
+-- := by subst_solve_hcompose Term, Ty, s, σ, τ
 
-instance instSubstMapHetCompose_TermTy : SubstMapHetCompose Term Ty where
-  apply_hcompose := Term.apply_hcompose
+-- instance instSubstMapHetCompose_TermTy : SubstMapHetCompose Term Ty where
+--   apply_hcompose := Term.apply_hcompose
 
-theorem Term.apply_id {t : Term} : t[+0] = t := by induction t; all_goals (simp at *; try simp [*])
+-- theorem Term.apply_id {t : Term} : t[+0] = t := by induction t; all_goals (simp at *; try simp [*])
 
-instance instSubstMapId_TermTy : SubstMapId Term Term where
-  apply_id := Term.apply_id
+-- instance instSubstMapId_TermTy : SubstMapId Term Term where
+--   apply_id := Term.apply_id
 
-theorem Term.apply_compose {s : Term} {σ τ : Subst Term} : s[σ][τ] = s[σ ∘ τ] := by
-  subst_solve_compose Term, s, σ, τ
+-- theorem Term.apply_compose {s : Term} {σ τ : Subst Term} : s[σ][τ] = s[σ ∘ τ] := by
+--   subst_solve_compose Term, s, σ, τ
 
-instance instSubstMapCompose_TermTerm : SubstMapCompose Term Term where
-  apply_compose := Term.apply_compose
-
-inductive IteratedSubst where
-| nil : IteratedSubst
-| term : Subst Term -> IteratedSubst -> IteratedSubst
-| type : Subst Ty -> IteratedSubst -> IteratedSubst
-
-def Term.isubst (t : Term) : IteratedSubst -> Term
-| .nil => t
-| .term σ tl => t[σ].isubst tl
-| .type σ tl => t[σ:Ty].isubst tl
+-- instance instSubstMapCompose_TermTerm : SubstMapCompose Term Term where
+--   apply_compose := Term.apply_compose
 
 end Surface
