Surface/Term.lean
@@ -1,4 +1,3 @@
 import Surface.Term.Definition
-import Surface.Term.Structure
 import Surface.Term.BEq
 import Surface.Term.Substitution
