Surface/Typing.lean
@@ -6,62 +6,64 @@ import Surface.Term
 import Surface.Global
 
 
-
 namespace Surface
 
-def KindEnv := List Kind
-def TyEnv := List Ty
+@[simp]
+abbrev KindEnv := List Kind
+
+@[simp]
+abbrev TyEnv := List Ty
 
 
-instance inst_getElem_TyEnv : GetElem TyEnv Nat Ty (λ env i => by simp [TyEnv] at env; apply i < env.length) where
-  getElem env i _ := by unfold TyEnv at env; apply env[i]
+-- instance inst_getElem_TyEnv : GetElem TyEnv Nat Ty (λ env i => by simp [TyEnv] at env; apply i < env.length) where
+--   getElem env i _ := by unfold TyEnv at env; apply env[i]
 
-instance inst_getElem?_TyEnv : GetElem? TyEnv Nat Ty
-         (λ env i => by simp [TyEnv] at env; apply i < env.length) where
-  getElem? env i := by unfold TyEnv at env; apply env[i]?
+-- instance inst_getElem?_TyEnv : GetElem? TyEnv Nat Ty
+--          (λ env i => by simp [TyEnv] at env; apply i < env.length) where
+--   getElem? env i := by unfold TyEnv at env; apply env[i]?
 
-instance inst_getElem_KindEnv : GetElem KindEnv Nat Kind
-         (λ env i => by simp [KindEnv] at env; apply i < env.length) where
-  getElem env i _ := by unfold KindEnv at env; apply env[i]
+-- instance inst_getElem_KindEnv : GetElem KindEnv Nat Kind
+--          (λ env i => by simp [KindEnv] at env; apply i < env.length) where
+--   getElem env i _ := by unfold KindEnv at env; apply env[i]
 
-instance inst_getElem?_KindEnv : GetElem? KindEnv Nat Kind
-         (λ env i => by simp [KindEnv] at env; apply i < env.length) where
-  getElem? env i := by unfold KindEnv at env; apply env[i]?
+-- instance inst_getElem?_KindEnv : GetElem? KindEnv Nat Kind
+--          (λ env i => by simp [KindEnv] at env; apply i < env.length) where
+--   getElem? env i := by unfold KindEnv at env; apply env[i]?
 
-def TyEnv.mapM [Monad m] (f : Ty -> m β) (env : TyEnv) := by simp [TyEnv] at env; apply env.mapM f
-def TyEnv.map (f : Ty -> β) (env : TyEnv) := by simp [TyEnv] at env; apply env.map f
+-- def TyEnv.mapM [Monad m] (f : Ty -> m β) (env : TyEnv) := by simp [TyEnv] at env; apply env.mapM f
+-- def TyEnv.map (f : Ty -> β) (env : TyEnv) := by simp [TyEnv] at env; apply env.map f
 
-def KindEnv.map (f : Kind -> β) (env : KindEnv) := by simp [KindEnv] at env; apply env.map f
-
-
-def ValidHeadVariable (t : Term) (test : String -> Bool) : Prop :=
-  ∃ x, Term.spine t = some x ∧ test x.fst
-
-def ValidTyHeadVariable (t : Ty) (test : String -> Bool) : Prop :=
-  ∃ x, Ty.spine t = some x ∧ test x.fst
-
-inductive StableTypeMatch : KindEnv -> Ty -> Ty -> Prop
-| refl :
-  Ty.spine R = some x ->
-  StableTypeMatch Δ R R
-| arrow :
-  StableTypeMatch Δ B R ->
-  StableTypeMatch Δ (A `-:> B) R
-| all :
-  StableTypeMatch (K::Δ) B R[+1] ->
-  StableTypeMatch Δ (`∀[K] B) R
+-- def KindEnv.map (f : Kind -> β) (env : KindEnv) := by simp [KindEnv] at env; apply env.map f
 
 
-inductive PrefixTypeMatch : KindEnv -> Ty -> Ty -> Ty -> Prop
-| refl :
-  Ty.spine B = some x ->
-  PrefixTypeMatch Δ B T T
-| arrow :
-  PrefixTypeMatch Δ B V T ->
-  PrefixTypeMatch Δ (A `-:> B) (A `-:> V) T
-| all :
-  PrefixTypeMatch (K::Δ) B V T[+1] ->
-  PrefixTypeMatch Δ (`∀[K] B) (`∀[K] V) T
+-- def ValidHeadVariable (t : Term) (test : String -> Bool) : Prop :=
+--   ∃ x, Term.spine t = some x ∧ test x.fst
+
+-- def ValidTyHeadVariable (t : Ty) (test : String -> Bool) : Prop :=
+--   ∃ x, Ty.spine t = some x ∧ test x.fst
+
+-- inductive StableTypeMatch : KindEnv -> Ty -> Ty -> Prop
+-- | refl :
+--   Ty.spine R = some x ->
+--   StableTypeMatch Δ R R
+-- | arrow :
+--   StableTypeMatch Δ B R ->
+--   StableTypeMatch Δ (A `-:> B) R
+-- | all :
+--   StableTypeMatch (K::Δ) B R[+1] ->
+--   StableTypeMatch Δ (`∀[K] B) R
+
+
+-- inductive PrefixTypeMatch : KindEnv -> Ty -> Ty -> Ty -> Prop
+-- | refl :
+--   Ty.spine B = some x ->
+--   PrefixTypeMatch Δ B T T
+-- | arrow :
+--   PrefixTypeMatch Δ B V T ->
+--   PrefixTypeMatch Δ (A `-:> B) (A `-:> V) T
+-- | all :
+--   PrefixTypeMatch (K::Δ) B V T[+1] ->
+--   PrefixTypeMatch Δ (`∀[K] B) (`∀[K] V) T
 
 
 inductive Kinding (G : GlobalEnv) : KindEnv -> Ty -> Kind -> Prop
